Use list-based vectors in the Imp compiler

examples/Imp2Vir/Combinators.v
@@ -4,14 +4,9 @@ From Coq Require Import
      Lists.List
      Strings.String
      Structures.OrderedTypeEx
-     Vector
      ZArith.
 
 Module Import StringMap := Coq.FSets.FMapList.Make(String_as_OT).
-Import VectorNotations.
-Import ListNotations.
-Open Scope Z_scope.
-Close Scope vector_scope.
 
 From ExtLib Require Import
      Structures.Monads
@@ -21,7 +16,13 @@ Import MonadNotation.
 From Vellvm Require Import
      Syntax.
 
-Require Import Imp.
+Import ListNotations.
+
+Require Import Imp Vector.
+Module Import Vec := Vector.
+
+Close Scope nat_scope.
+Open Scope Z_scope.
 
 Section compile_cvir.
 
@@ -54,7 +55,7 @@ Fixpoint compile_expr (next_reg:int) (e: expr) (env: StringMap.t int): option (i
   | Lit n => Some(next_reg, [(IId (Anon next_reg), INSTR_Op (EXP_Integer (Z.of_nat n)))])
   | Plus e1 e2 =>
     '(reg1, instrs1) <- compile_expr next_reg e1 env;;
-    '(reg2, instrs2) <- compile_expr (reg1 + 1) e2 env;;
+    '(reg2, instrs2) <- compile_expr (reg1 + 1)%Z e2 env;;
     ret (reg2 + 1, instrs1 ++ instrs2 ++ compile_binop reg1 reg2 (reg2 + 1) (Add false false))
   | Minus e1 e2 =>
     '(reg1, instrs1) <- compile_expr next_reg e1 env;;
@@ -82,18 +83,18 @@ Definition compile_assign (next_reg : int) (x: Imp.var) (e: expr) (env : StringM
 Record cvir (n_in n_out : nat) : Type := {
    n_int : nat;
    blocks : forall
-     (v_in : Vector.t int n_in)
-     (v_out : Vector.t int n_out)
-     (v_int : Vector.t int n_int),
+     (v_in : Vec.t int n_in)
+     (v_out : Vec.t int n_out)
+     (v_int : Vec.t int n_int),
      list (block typ);
 }.
 
 Definition mk_cvir
   {n_in n_out n_int : nat}
   (blocks : forall
-    (v_in : Vector.t int n_in)
-    (v_out : Vector.t int n_out)
-    (v_int : Vector.t int n_int),
+    (v_in : Vec.t int n_in)
+    (v_out : Vec.t int n_out)
+    (v_int : Vec.t int n_int),
     list (block typ)
   ) :
   cvir n_in n_out :=
@@ -102,23 +103,23 @@ Definition mk_cvir
     blocks := blocks
   |}.
 
-Arguments n_int : default implicits.
-Arguments blocks : default implicits.
+Arguments n_int {_} {_}.
+Arguments blocks {_} {_}.
 
 Definition block_cvir (c : code typ) : cvir 1 1 :=
   mk_cvir (fun
-    (vi : Vector.t int 1)
-    (vo : Vector.t int 1)
-    (vt : Vector.t int 0)
-    => [mk_block (Anon (hd vi)) (List.nil) c (TERM_Br_1 (Anon (hd vo))) None]
+    (vi : Vec.t int 1)
+    (vo : Vec.t int 1)
+    (vt : Vec.t int 0)
+    => [mk_block (Anon (Vec.hd vi)) (List.nil) c (TERM_Br_1 (Anon (hd vo))) None]
   ).
 
 Definition branch_cvir (c : code typ) (e : texp typ) : cvir 1 2 :=
   mk_cvir (fun
-    (vi : Vector.t int 1)
-    (vo : Vector.t int 2)
-    (vt : Vector.t int 0)
-    => [mk_block (Anon (hd vi)) (List.nil) c (TERM_Br e (Anon (hd vo)) (Anon (hd (tl vo)))) None]
+    (vi : Vec.t int 1)
+    (vo : Vec.t int 2)
+    (vt : Vec.t int 0)
+    => [mk_block (Anon (Vec.hd vi)) (List.nil) c (TERM_Br e (Anon (Vec.hd vo)) (Anon (Vec.hd (Vec.tl vo)))) None]
   ).
 
 Definition merge_cvir
@@ -127,9 +128,9 @@ Definition merge_cvir
   (b2: cvir ni2 no2) :
   cvir (ni1+ni2) (no1+no2) :=
     mk_cvir (fun vi vo vt =>
-      let '(li,ri) := Vector.splitat ni1 vi in
-      let '(lo,ro) := Vector.splitat no1 vo in
-      let '(lt,rt) := Vector.splitat (n_int b1) vt in
+      let '(li,ri) := Vec.splitat ni1 vi in
+      let '(lo,ro) := Vec.splitat no1 vo in
+      let '(lt,rt) := Vec.splitat (n_int b1) vt in
       (blocks b1 li lo lt) ++ (blocks b2 ri ro rt)
     ).
 
@@ -137,8 +138,8 @@ Definition seq_cvir {ni1 no1 ni2 no2 : nat}
   (b1 : cvir ni1 (S no1))
   (b2: cvir (S ni2) no2) :
   cvir (ni1+ni2) (no1+no2) :=
-    mk_cvir (fun vi vo (vt : Vector.t int (S (n_int b1 + n_int b2))) =>
-      let '(newint,vt) := Vector.uncons vt in
+    mk_cvir (fun vi vo (vt : Vec.t int (S (n_int b1 + n_int b2))) =>
+      let '(newint,vt) := Vec.uncons vt in
       let b1 := mk_cvir (fun vi vo vt => (blocks b1) vi (newint :: vo)%vector vt) in
       let b2 := mk_cvir (fun vi vo vt => (blocks b2) (newint :: vi)%vector vo vt) in
       blocks (merge_cvir b1 b2) vi vo vt
@@ -146,7 +147,7 @@ Definition seq_cvir {ni1 no1 ni2 no2 : nat}
 
 Definition loop_cvir {ni no : nat} (b : cvir (S ni) (S no)) : cvir ni no :=
   mk_cvir (fun vi vo vt =>
-    let '(newint,vt) := Vector.uncons vt in
+    let '(newint,vt) := Vec.uncons vt in
     (blocks b) (newint :: vi)%vector (newint :: vo)%vector vt
   ).
 
@@ -157,7 +158,7 @@ Definition loop_cvir_open {ni no : nat} (b : cvir (S ni) (S no)) : cvir (S ni) n
 
 Definition join_cvir {ni no : nat} (b : cvir ni (S (S no))) : cvir ni (S no) :=
   mk_cvir (fun vi vo vt =>
-    let '(o, vo) := Vector.uncons vo in
+    let '(o, vo) := Vec.uncons vo in
     (blocks b) vi (o :: o :: vo)%vector vt
   ).
 
@@ -185,7 +186,7 @@ Fixpoint compile (next_reg : int) (s : stmt) (env: StringMap.t int)
       | Some (next_reg, _, ir) => let br := branch_cvir expr_ir (texp_i32 expr_reg) in
         let body := seq_cvir br ir in
         let ir := loop_cvir_open body in
-        let ir := mk_cvir (fun vi vo vt => (blocks ir) vi (rev vo) vt) in
+        let ir := mk_cvir (fun vi vo vt => (blocks ir) vi (* rev *) vo vt) in
         ret (next_reg, env, ir)
       end
   (*| If e l r =>
@@ -197,56 +198,11 @@ Fixpoint compile (next_reg : int) (s : stmt) (env: StringMap.t int)
   | _ => None
   end.
 
-Definition fact_ir := (compile 0 (fact "a" "b" 5) (empty int)).
+Definition fact_ir := (compile 0 (fact "a" "b" 5) (StringMap.empty int)).
 
-Eval compute in match fact_ir with
+(*Eval compute in match fact_ir with
 | None => None
 | Some (_,_,ir) => Some ((blocks ir) [-1]%vector [-1]%vector (const (-1)%Z (n_int ir)))
-end.
-
-
-Definition unique_vector {A} {n} (v : Vector.t A n) : Prop :=
-  forall i1 i2, nth v i1 = nth v i2 -> i1 = i2.
-
-Definition unique_bid {ni no} ir : Prop :=
-  forall (vi : Vector.t int ni) (vo : Vector.t int no) vt,
-  forall b1 b2,
-  unique_vector (append vi vt) ->
-  List.In b1 (blocks ir vi vo vt) ->
-  List.In b2 (blocks ir vi vo vt) ->
-  blk_id b1 = blk_id b2 ->
-  b1 = b2.
-
-Theorem merge_cvir_unique :
-  forall ni1 no1 ni2 no2 (ir1 : cvir ni1 no1) (ir2 : cvir ni2 no2),
-  unique_bid ir1 -> unique_bid ir2 -> unique_bid (merge_cvir ir1 ir2).
-Proof.
-  intros.
-  simpl in *.
-  unfold unique_bid in *.
-  unfold unique_vector in *.
-  simpl in *.
-  intros.
-  destruct (splitat ni1 _) eqn:? in *.
-  destruct (splitat no1 _) eqn:? in *.
-  destruct (splitat (n_int _) _) eqn:? in *.
-  apply append_splitat in Heqp, Heqp0, Heqp1.
-  subst.
-  apply in_app_iff in H2, H3.
-  destruct H2, H3.
-  - eapply H.
-    intros.
-    2,3,4: eassumption.
-    assert (i1' := Fin.L (ni2 + n_int ir2) i1).
-    assert (i2' := Fin.L (ni2 + n_int ir2) i2).
-    assert (ni1 + n_int ir1 + (ni2 + n_int ir2) = ni1 + ni2 + (n_int ir1 + n_int ir2))%nat. lia.
-    assert (i1'' := Fin.cast i1' H6).
-    assert (i2'' := Fin.cast i1' H6).
-    specialize (H1 i1'' i2'').
-    Search (_ = _ -> _ _ = _ _).
-    assert (i1'' = i2'').
-    admit. (* in_app_iff *)
-    admit. (* Fin.L/Fin.cast injective *)
-Admitted.
+end.*)
 
 End compile_cvir.
