examples/Imp2Vir/CombinatorsWF.v
@@ -1,0 +1,93 @@
+From Coq Require Import
+     Lia
+     List
+     NArith.
+
+From Vellvm Require Import Syntax.
+
+From tutorial Require Import Fin.
+
+Require Import Vector Combinators.
+
+Open Scope nat_scope.
+Open Scope vector_scope.
+
+Arguments n_int : default implicits.
+Arguments blocks : default implicits.
+
+Definition unique_vector {A} {n} (v : Vector.t A n) : Prop :=
+  forall i1 i2, nth v i1 = nth v i2 -> i1 = i2.
+
+Definition unique_bid {ni no} ir : Prop :=
+  forall (vi : Vector.t int ni) (vo : Vector.t int no) vt,
+  forall b1 b2,
+  unique_vector (vi ++ vt)%vector ->
+  List.In b1 (blocks ir vi vo vt) ->
+  List.In b2 (blocks ir vi vo vt) ->
+  blk_id b1 = blk_id b2 ->
+  b1 = b2.
+
+Theorem vector_in_app_iff : forall A n n' (v : Vector.t A n) (v' : Vector.t A n') (a : A),
+  Vector.In a (v ++ v')%vector <-> Vector.In a v \/ Vector.In a v'.
+Proof.
+  intros ? ? ? [] [] ?.
+  unfold In in *. simpl in *.
+  apply in_app_iff.
+Qed.
+
+Theorem nth_firstn : forall A (l : list A) i n (H : i < n) a,
+  List.nth i l a = List.nth i (firstn n l) a.
+Admitted.
+
+Theorem merge_cvir_unique :
+  forall ni1 no1 ni2 no2 (ir1 : cvir ni1 no1) (ir2 : cvir ni2 no2),
+  unique_bid ir1 -> unique_bid ir2 -> unique_bid (merge_cvir ir1 ir2).
+Proof.
+  unfold unique_bid.
+  unfold unique_vector.
+  intros.
+  apply in_app_iff in H2, H3.
+  simpl in *.
+  destruct H2, H3.
+  - eapply H.
+    2,3,4: eassumption.
+    intros.
+    destruct vi, vo, vt, i1, i2.
+    apply Fin.unique_fin.
+    simpl in *.
+    unfold Vec.append in *.
+    simpl in *.
+    erewrite nth_rewrite in H5.
+    erewrite nth_rewrite in H5.
+    simpl in H5.
+    assert (x2 < length (firstn ni1 x) \/ x2 >= length (firstn ni1 x)).
+    lia.
+    assert (x3 < length (firstn ni1 x) \/ x3 >= length (firstn ni1 x)).
+    lia.
+    destruct H6, H7.
+    + erewrite 2 app_nth1 in H5 ; try assumption.
+      rewrite firstn_length in H6,H7.
+      epose (x2' := fi' x2). epose (x3' := fi' x3).
+      specialize (H1 x2' x3').
+      erewrite 2 nth_rewrite in H1.
+      simpl in H1.
+      rewrite 2 app_nth1 in H1 ; try lia.
+      rewrite<- 2 nth_firstn in H5 ; try lia.
+      apply H1 in H5.
+      injection H5 as ?.
+      exact H5.
+   + erewrite app_nth1 in H5 ; try assumption.
+     erewrite app_nth2 in H5 ; try assumption.
+     rewrite firstn_length in H5,H6,H7.
+     epose (x2' := fi' x2). epose (x3' := fi' (ni2 + x3)).
+     specialize (H1 x2' x3').
+     erewrite 2 nth_rewrite in H1.
+     simpl in H1.
+     rewrite app_nth1 in H1 ; try lia.
+     rewrite app_nth2 in H1 ; try lia.
+     rewrite<- 2 nth_firstn in H5 ; try lia.
+     rewrite min_l in H5 ; try lia.
+     replace (x3 - ni1) with (ni2 + x3 - length x ) in H5 by lia.
+     apply H1 in H5.
+     injection H5 as ?.
+Admitted.
