examples/Imp2Vir/Vector.v
@@ -1,0 +1,153 @@
+From Coq Require Import
+     Lia
+     Lists.List
+     Arith
+     ZArith.
+
+From Vellvm Require Import
+     Syntax.
+
+From tutorial Require Import Fin.
+
+Section Vector.
+
+Open Scope nat_scope.
+
+Definition t (A : Type) (n : nat) : Type := { l : list A | length l = n }.
+
+Notation vec' l := (exist (fun l' : list _ => _) l _).
+
+Theorem vector_proj1_unique : forall A n (v v' : t A n),
+    proj1_sig v = proj1_sig v' -> v = v'.
+Proof.
+  intros.
+  destruct v, v'.
+  simpl in *.
+  destruct H.
+  f_equal.
+  subst. rewrite Eqdep_dec.UIP_refl_nat.
+  reflexivity.
+Qed.
+
+Program Definition empty (A : Type) : t A 0 := vec' nil.
+
+Program Definition cons {A} {n} h (v : t A n) : t A (S n) := vec' (h::v).
+Next Obligation.
+  destruct v. simpl in *.
+  f_equal.
+  assumption.
+Defined.
+
+Program Definition hd {A} {n} (v : t A (S n)) : A :=
+  match proj1_sig v with
+  | h :: _ => h
+  | nil => _
+  end.
+Next Obligation.
+  destruct v.
+  destruct x.
+  - discriminate e.
+  - exact a.
+Qed.
+
+Program Definition tl {A} {n} (v : t A (S n)) : t A n :=
+  match proj1_sig v with
+  | _ :: v' => vec' v'
+  | nil => _
+  end.
+Next Obligation.
+  destruct v.
+  simpl in *. subst. simpl in e. injection e as e. exact e.
+Defined.
+Next Obligation.
+  destruct v.
+  destruct x.
+  - discriminate e.
+  - simpl in *. discriminate Heq_anonymous.
+Qed.
+
+Program Definition nth {A} {n} (v : t A n) (i : fin n) : A :=
+  match proj1_sig v with
+  | h :: l => List.nth i v h
+  | nil => _
+  end.
+Next Obligation.
+  destruct n. destruct i.
+  - lia.
+  - destruct v. simpl in *. subst. discriminate e.
+Qed.
+
+Theorem nth_rewrite : forall A n (v : t A n) i a, nth v i = List.nth (proj1_sig i) (proj1_sig v) a.
+Proof.
+  intros ? ? [] [] ?.
+  subst.
+  simpl.
+  unfold nth. simpl. destruct x eqn:?.
+  - simpl in l. lia.
+  - subst. rewrite (nth_indep _ a a0 l). reflexivity.
+Qed.
+
+(*Definition unique_vector {A} {n} (v : t A n) : Prop :=
+  forall i1 i2, nth v i1 = nth v i2 -> i1 = i2.*)
+
+Program Definition append {A} {n n'} (v : t A n) (v' : t A n') :
+  t A (n + n') := vec' ((proj1_sig v) ++ proj1_sig v').
+Next Obligation.
+  rewrite app_length. destruct v, v'. simpl. subst. reflexivity.
+Defined.
+
+Definition In {A} {n} a (v : t A n) := List.In a (proj1_sig v).
+
+Program Definition splitat {A} i {j} (v : t A (i+j)) :
+  t A i * t A j :=
+  (vec' (firstn i (proj1_sig v)), vec' (skipn i (proj1_sig v))).
+Next Obligation.
+  destruct v. simpl in *. rewrite firstn_length. rewrite e.
+  rewrite (plus_n_O i) at 1. rewrite Nat.add_min_distr_l. rewrite Nat.min_0_l.
+  apply Nat.add_0_r.
+Defined.
+Next Obligation.
+  destruct v. simpl in *. rewrite skipn_length. apply Nat.add_sub_eq_l. auto.
+Defined.
+
+Theorem append_splitat : forall A n n' (v : t A n) (v' : t A n') (v'' : t A (n+n')),
+  splitat n v'' = (v, v') -> v'' = append v v'.
+Proof.
+  intros.
+  destruct v, v', v''.
+  unfold splitat, append in *.
+  simpl in *.
+  injection H as ?.
+  subst x x0.
+  apply vector_proj1_unique. simpl.
+  rewrite (firstn_skipn n x1).
+  reflexivity.
+Qed.
+
+Program Definition uncons {A} {n} (v : t A (S n)) : A * t A n :=
+  match proj1_sig v with
+  | a :: t => (a, vec' t)
+  | _ => _
+  end.
+Next Obligation.
+  destruct v as [[] ?].
+  discriminate e.
+  simpl in *.
+  injection Heq_anonymous as ?.
+  subst.
+  auto.
+Defined.
+Next Obligation.
+  destruct v as [[] ?].
+  discriminate e.
+  simpl in *. injection e as ?.
+  refine (a, vec' l). exact H0.
+Defined.
+
+End Vector.
+
+Declare Scope vector_scope.
+Delimit Scope vector_scope with vector.
+Notation "h :: t" := (cons h t) (at level 60, right associativity).
+Infix "++" := append : vector_scope.
+Notation vec' l := (exist (fun l' : list _ => _) l _).
